examples/ghc/lib/Id.v
@@ -17,25 +17,35 @@ Require Coq.Program.Wf.
 (* Converted imports: *)
 
 Require BasicTypes.
-Require CoreSyn.
+Require Class.
 Require DataCon.
+Require Datatypes.
 Require Demand.
 Require FastString.
+Require GHC.Base.
+Require GHC.Enum.
+Require GHC.List.
 Require GHC.Num.
 Require IdInfo.
+Require Maybes.
 Require Module.
 Require Name.
 Require OccName.
+Require Panic.
 Require SrcLoc.
 Require UniqSupply.
 Require Unique.
+Require Util.
 Require Var.
+Import GHC.Base.Notations.
+Import GHC.Num.Notations.
 
 (* No type declarations to convert. *)
 (* Midamble *)
 
-(* Record selectors *)
-Import IdInfo.
+Parameter lookupDataCon : IdInfo.DataConId -> DataCon.DataCon.
+Parameter lookupClass : IdInfo.ClassId -> Class.Class.
+
 
 (*
 Parameter hasNoBinding : Var.Id -> bool.
@@ -91,249 +101,525 @@ Parameter setIdType : Var.Id -> Core.Type_ -> Var.Id.
 *)
 (* Converted value declarations: *)
 
-Axiom idIsFrom : Module.Module -> Var.Id -> bool.
-
-Axiom localiseId : Var.Id -> Var.Id.
-
-Axiom idName : Var.Id -> Name.Name.
-
-Axiom idUnique : Var.Id -> Unique.Unique.
-
-Axiom isProbablyOneShotLambda : Var.Id -> bool.
-
-Axiom isOneShotBndr : Var.Var -> bool.
-
-Axiom idStateHackOneShotInfo : Var.Id -> BasicTypes.OneShotInfo.
-
-(* isStrictId skipped *)
-
-Axiom idFunRepArity : Var.Id -> BasicTypes.RepArity.
-
-(* isDictId skipped *)
-
-Axiom idType : Var.Id -> unit.
-
-Axiom setIdName : Var.Id -> Name.Name -> Var.Id.
-
-Axiom setIdUnique : Var.Id -> Unique.Unique -> Var.Id.
-
-(* setIdType skipped *)
-
-Axiom setIdExported : Var.Id -> Var.Id.
-
-Axiom setIdNotExported : Var.Id -> Var.Id.
-
-Axiom asJoinId_maybe : Var.Id -> option BasicTypes.JoinArity -> Var.Id.
-
-Axiom zapJoinId : Var.Id -> Var.Id.
-
-Axiom zapIdTailCallInfo : Var.Id -> Var.Id.
-
-Axiom zapIdUsedOnceInfo : Var.Id -> Var.Id.
-
-Axiom zapIdUsageEnvInfo : Var.Id -> Var.Id.
-
-Axiom zapIdUsageInfo : Var.Id -> Var.Id.
-
-Axiom zapIdDemandInfo : Var.Id -> Var.Id.
-
-Axiom zapFragileIdInfo : Var.Id -> Var.Id.
-
-Axiom zapLamIdInfo : Var.Id -> Var.Id.
-
-Axiom zapInfo : (IdInfo.IdInfo -> option IdInfo.IdInfo) -> Var.Id -> Var.Id.
-
-Axiom maybeModifyIdInfo : option IdInfo.IdInfo -> Var.Id -> Var.Id.
-
-Axiom transferPolyIdInfo : Var.Id -> list Var.Var -> Var.Id -> Var.Id.
-
-Axiom updOneShotInfo : Var.Id -> BasicTypes.OneShotInfo -> Var.Id.
-
-Axiom setIdOneShotInfo : Var.Id -> BasicTypes.OneShotInfo -> Var.Id.
-
-Axiom clearOneShotLambda : Var.Id -> Var.Id.
-
-Axiom setOneShotLambda : Var.Id -> Var.Id.
-
-Axiom setInlineActivation : Var.Id -> BasicTypes.Activation -> Var.Id.
-
-Axiom modifyInlinePragma : Var.Id ->
-                           (BasicTypes.InlinePragma -> BasicTypes.InlinePragma) -> Var.Id.
-
-Axiom setInlinePragma : Var.Id -> BasicTypes.InlinePragma -> Var.Id.
-
-Axiom zapIdOccInfo : Var.Id -> Var.Id.
-
-Axiom setIdOccInfo : Var.Id -> BasicTypes.OccInfo -> Var.Id.
-
-Axiom setIdCafInfo : Var.Id -> IdInfo.CafInfo -> Var.Id.
-
-Axiom setIdSpecialisation : Var.Id -> IdInfo.RuleInfo -> Var.Id.
-
-Axiom setIdDemandInfo : Var.Id -> Demand.Demand -> Var.Id.
-
-Axiom zapStableUnfolding : Var.Id -> Var.Id.
-
-Axiom setCaseBndrEvald : DataCon.StrictnessMark -> Var.Id -> Var.Id.
-
-Axiom setIdUnfolding : Var.Id -> CoreSyn.Unfolding -> Var.Id.
-
-Axiom zapIdStrictness : Var.Id -> Var.Id.
-
-Axiom setIdStrictness : Var.Id -> Demand.StrictSig -> Var.Id.
-
-Axiom setIdCallArity : Var.Id -> BasicTypes.Arity -> Var.Id.
-
-Axiom setIdArity : Var.Id -> BasicTypes.Arity -> Var.Id.
-
-Axiom modifyIdInfo : (IdInfo.IdInfo -> IdInfo.IdInfo) -> Var.Id -> Var.Id.
-
-Axiom setIdInfo : Var.Id -> IdInfo.IdInfo -> Var.Id.
-
-Axiom lazySetIdInfo : Var.Id -> IdInfo.IdInfo -> Var.Id.
-
-(* mkVanillaGlobal skipped *)
-
-(* mkVanillaGlobalWithInfo skipped *)
-
-Axiom mkGlobalId : IdInfo.IdDetails ->
-                   Name.Name -> unit -> IdInfo.IdInfo -> Var.Id.
-
-Axiom mkUserLocal : OccName.OccName ->
-                    Unique.Unique -> unit -> SrcLoc.SrcSpan -> Var.Id.
-
-Axiom mkSysLocalM : forall {m},
-                    forall `{UniqSupply.MonadUnique m}, FastString.FastString -> unit -> m Var.Id.
-
-Axiom mkSysLocal : FastString.FastString -> Unique.Unique -> unit -> Var.Id.
-
-Axiom mkWorkerId : Unique.Unique -> Var.Id -> unit -> Var.Id.
-
-Axiom mkUserLocalOrCoVar : OccName.OccName ->
-                           Unique.Unique -> unit -> SrcLoc.SrcSpan -> Var.Id.
-
-Axiom mkTemplateLocals : list unit -> list Var.Id.
-
-(* mkTemplateLocalsNum skipped *)
-
-Axiom mkTemplateLocal : GHC.Num.Int -> unit -> Var.Id.
-
-Axiom mkSysLocalOrCoVarM : forall {m},
-                           forall `{UniqSupply.MonadUnique m}, FastString.FastString -> unit -> m Var.Id.
-
-Axiom mkSysLocalOrCoVar : FastString.FastString ->
-                          Unique.Unique -> unit -> Var.Id.
-
-(* mkLocalIdOrCoVar skipped *)
-
-(* mkLocalId skipped *)
-
-(* mkLocalCoVar skipped *)
-
-(* mkLocalIdOrCoVarWithInfo skipped *)
-
-(* mkLocalIdWithInfo skipped *)
-
-Axiom mkExportedLocalId : IdInfo.IdDetails -> Name.Name -> unit -> Var.Id.
-
-(* mkExportedVanillaId skipped *)
-
-Axiom recordSelectorTyCon : Var.Id -> IdInfo.RecSelParent.
-
-Axiom isRecordSelector : Var.Id -> bool.
-
-Axiom isDataConRecordSelector : Var.Id -> bool.
-
-Axiom isPatSynRecordSelector : Var.Id -> bool.
-
-Axiom isNaughtyRecordSelector : Var.Id -> bool.
-
-(* isClassOpId_maybe skipped *)
-
-(* isPrimOpId skipped *)
-
-Axiom isDFunId : Var.Id -> bool.
-
-(* isPrimOpId_maybe skipped *)
-
-(* isFCallId skipped *)
-
-(* isFCallId_maybe skipped *)
-
-(* isConLikeId skipped *)
-
-(* isDataConWorkId skipped *)
-
-(* isDataConWorkId_maybe skipped *)
-
-(* idDataCon skipped *)
-
-(* isDataConId_maybe skipped *)
-
-Axiom isExitJoinId : Var.Var -> bool.
-
-Axiom isJoinId : Var.Var -> bool.
-
-Axiom idJoinArity : Var.JoinId -> BasicTypes.JoinArity.
-
-Axiom isJoinId_maybe : Var.Var -> option BasicTypes.JoinArity.
-
-(* hasNoBinding skipped *)
-
-Axiom isImplicitId : Var.Id -> bool.
-
-(* isDeadBinder skipped *)
-
-(* isEvVar skipped *)
-
-Axiom asJoinId : Var.Id -> BasicTypes.JoinArity -> Var.JoinId.
-
-(* idArity skipped *)
-
-(* idCallArity skipped *)
-
-(* isBottomingId skipped *)
-
-(* idStrictness skipped *)
-
-Axiom idUnfolding : Var.Id -> CoreSyn.Unfolding.
-
-Axiom realIdUnfolding : Var.Id -> CoreSyn.Unfolding.
-
-(* idDemandInfo skipped *)
-
-(* idHasRules skipped *)
-
-(* idCoreRules skipped *)
-
-(* idSpecialisation skipped *)
-
-(* idCafInfo skipped *)
-
-(* idOccInfo skipped *)
-
-(* idRuleMatchInfo skipped *)
-
-(* idInlineActivation skipped *)
-
-(* idInlinePragma skipped *)
-
-(* idOneShotInfo skipped *)
-
-(* typeOneShot skipped *)
-
-Axiom stateHackOneShot : BasicTypes.OneShotInfo.
-
-(* isStateHackType skipped *)
-
-Axiom isNeverLevPolyId : Var.Id -> bool.
+Definition asJoinId : Var.Id -> BasicTypes.JoinArity -> Var.JoinId :=
+  fun id arity =>
+    let is_vanilla_or_join :=
+      fun id =>
+        match Var.idDetails id with
+        | IdInfo.VanillaId => true
+        | IdInfo.JoinId _ => true
+        | _ => false
+        end in
+    Panic.warnPprTrace (negb (Var.isLocalId id)) (GHC.Base.hs_string__
+                        "ghc/compiler/basicTypes/Id.hs") #590 (GHC.Base.mappend (Datatypes.id
+                                                                                 (GHC.Base.hs_string__
+                                                                                  "global id being marked as join var:"))
+                                                                                (Panic.noString id)) (Panic.warnPprTrace
+                                                                                                      (negb
+                                                                                                       (is_vanilla_or_join
+                                                                                                        id))
+                                                                                                      (GHC.Base.hs_string__
+                                                                                                       "ghc/compiler/basicTypes/Id.hs")
+                                                                                                      #592
+                                                                                                      (GHC.Base.mappend
+                                                                                                       (Panic.noString
+                                                                                                        id)
+                                                                                                       Panic.someSDoc)
+                                                                                                      (Var.setIdDetails
+                                                                                                       id (IdInfo.JoinId
+                                                                                                        arity))).
+
+Definition hasNoBinding : Var.Id -> bool :=
+  fun id =>
+    match Var.idDetails id with
+    | IdInfo.PrimOpId _ => true
+    | IdInfo.FCallId _ => true
+    | IdInfo.DataConWorkId dc =>
+        orb (DataCon.isUnboxedTupleCon (lookupDataCon dc)) (DataCon.isUnboxedSumCon
+             (lookupDataCon dc))
+    | _ => false
+    end.
+
+Definition idArity : Var.Id -> BasicTypes.Arity :=
+  fun id => IdInfo.arityInfo ((@Var.idInfo tt id)).
+
+Definition idCafInfo : Var.Id -> IdInfo.CafInfo :=
+  fun id => IdInfo.cafInfo ((@Var.idInfo tt id)).
+
+Definition idCallArity : Var.Id -> BasicTypes.Arity :=
+  fun id => IdInfo.callArityInfo ((@Var.idInfo tt id)).
+
+Definition idInlinePragma : Var.Id -> BasicTypes.InlinePragma :=
+  fun id => IdInfo.inlinePragInfo ((@Var.idInfo tt id)).
+
+Definition idRuleMatchInfo : Var.Id -> BasicTypes.RuleMatchInfo :=
+  fun id => BasicTypes.inlinePragmaRuleMatchInfo (idInlinePragma id).
+
+Definition idInlineActivation : Var.Id -> BasicTypes.Activation :=
+  fun id => BasicTypes.inlinePragmaActivation (idInlinePragma id).
+
+Definition idName : Var.Id -> Name.Name :=
+  Var.varName.
+
+Definition localiseId : Var.Id -> Var.Id :=
+  fun id =>
+    let name := idName id in
+    if (if false : bool
+        then (Panic.assertPanic (GHC.Base.hs_string__ "ghc/compiler/basicTypes/Id.hs")
+              #209)
+        else andb (Var.isLocalId id) (Name.isInternalName name)) : bool
+    then id else
+    Var.mkLocalVar (Var.idDetails id) (Name.localiseName name) (tt) ((@Var.idInfo tt
+                                                                      id)).
+
+Definition idIsFrom : Module.Module -> Var.Id -> bool :=
+  fun mod_ id => Name.nameIsLocalOrFrom mod_ (idName id).
+
+Definition idOccInfo : Var.Id -> BasicTypes.OccInfo :=
+  fun id => IdInfo.occInfo ((@Var.idInfo tt id)).
+
+Definition isDeadBinder : Var.Id -> bool :=
+  fun bndr =>
+    if Var.isId bndr : bool then BasicTypes.isDeadOcc (idOccInfo bndr) else
+    false.
+
+Definition idOneShotInfo : Var.Id -> BasicTypes.OneShotInfo :=
+  fun id => IdInfo.oneShotInfo ((@Var.idInfo tt id)).
+
+Definition idSpecialisation : Var.Id -> IdInfo.RuleInfo :=
+  fun id => IdInfo.ruleInfo ((@Var.idInfo tt id)).
+
+Definition idHasRules : Var.Id -> bool :=
+  fun id => negb (IdInfo.isEmptyRuleInfo (idSpecialisation id)).
+
+Definition idType : Var.Id -> unit :=
+  Var.varType.
+
+Definition idUnique : Var.Id -> Unique.Unique :=
+  Var.varUnique.
+
+Definition isClassOpId_maybe : Var.Id -> option Class.Class :=
+  fun id =>
+    match Var.idDetails id with
+    | IdInfo.ClassOpId cls => Some (lookupClass cls)
+    | _other => None
+    end.
+
+Definition isDFunId : Var.Id -> bool :=
+  fun id =>
+    match Var.idDetails id with
+    | IdInfo.DFunId _ => true
+    | _ => false
+    end.
+
+Definition isDataConId_maybe : Var.Id -> option DataCon.DataCon :=
+  fun id =>
+    match Var.idDetails id with
+    | IdInfo.DataConWorkId con => Some (lookupDataCon con)
+    | IdInfo.DataConWrapId con => Some (lookupDataCon con)
+    | _ => None
+    end.
+
+Definition idDataCon : Var.Id -> DataCon.DataCon :=
+  fun id =>
+    Maybes.orElse (isDataConId_maybe id) (Panic.panicStr (GHC.Base.hs_string__
+                                                          "idDataCon") (Panic.noString id)).
+
+Definition isDataConRecordSelector : Var.Id -> bool :=
+  fun id =>
+    match Var.idDetails id with
+    | IdInfo.RecSelId (IdInfo.RecSelData _) _ => true
+    | _ => false
+    end.
+
+Definition isDataConWorkId : Var.Id -> bool :=
+  fun id =>
+    match Var.idDetails id with
+    | IdInfo.DataConWorkId _ => true
+    | _ => false
+    end.
+
+Definition isConLikeId : Var.Id -> bool :=
+  fun id => orb (isDataConWorkId id) (BasicTypes.isConLike (idRuleMatchInfo id)).
+
+Definition isDataConWorkId_maybe : Var.Id -> option DataCon.DataCon :=
+  fun id =>
+    match Var.idDetails id with
+    | IdInfo.DataConWorkId con => Some (lookupDataCon con)
+    | _ => None
+    end.
+
+Definition isFCallId : Var.Id -> bool :=
+  fun id =>
+    match Var.idDetails id with
+    | IdInfo.FCallId _ => true
+    | _ => false
+    end.
+
+Definition isFCallId_maybe : Var.Id -> option unit :=
+  fun id =>
+    match Var.idDetails id with
+    | IdInfo.FCallId call => Some call
+    | _ => None
+    end.
+
+Definition isImplicitId : Var.Id -> bool :=
+  fun id =>
+    match Var.idDetails id with
+    | IdInfo.FCallId _ => true
+    | IdInfo.ClassOpId _ => true
+    | IdInfo.PrimOpId _ => true
+    | IdInfo.DataConWorkId _ => true
+    | IdInfo.DataConWrapId _ => true
+    | _ => false
+    end.
+
+Definition isJoinId : Var.Var -> bool :=
+  fun id =>
+    if Var.isId id : bool
+    then match Var.idDetails id with
+         | IdInfo.JoinId _ => true
+         | _ => false
+         end else
+    false.
+
+Definition isExitJoinId : Var.Var -> bool :=
+  fun id =>
+    andb (isJoinId id) (andb (BasicTypes.isOneOcc (idOccInfo id))
+                             (BasicTypes.occ_in_lam (idOccInfo id))).
+
+Definition isJoinId_maybe : Var.Var -> option BasicTypes.JoinArity :=
+  fun id =>
+    if Var.isId id : bool
+    then if false : bool
+         then (None)
+         else match Var.idDetails id with
+              | IdInfo.JoinId arity => Some arity
+              | _ => None
+              end else
+    None.
+
+Definition idJoinArity : Var.JoinId -> BasicTypes.JoinArity :=
+  fun id =>
+    Maybes.orElse (isJoinId_maybe id) (Panic.panicStr (GHC.Base.hs_string__
+                                                       "idJoinArity") (Panic.noString id)).
+
+Definition isNaughtyRecordSelector : Var.Id -> bool :=
+  fun id =>
+    match Var.idDetails id with
+    | IdInfo.RecSelId _ n => n
+    | _ => false
+    end.
+
+Definition isPatSynRecordSelector : Var.Id -> bool :=
+  fun id =>
+    match Var.idDetails id with
+    | IdInfo.RecSelId (IdInfo.RecSelPatSyn _) _ => true
+    | _ => false
+    end.
+
+Definition isPrimOpId : Var.Id -> bool :=
+  fun id =>
+    match Var.idDetails id with
+    | IdInfo.PrimOpId _ => true
+    | _ => false
+    end.
+
+Definition isPrimOpId_maybe : Var.Id -> option unit :=
+  fun id =>
+    match Var.idDetails id with
+    | IdInfo.PrimOpId op => Some op
+    | _ => None
+    end.
+
+Definition isRecordSelector : Var.Id -> bool :=
+  fun id =>
+    match Var.idDetails id with
+    | IdInfo.RecSelId _ _ => true
+    | _ => false
+    end.
+
+Definition lazySetIdInfo : Var.Id -> IdInfo.IdInfo -> Var.Id :=
+  Var.lazySetIdInfo.
+
+Definition maybeModifyIdInfo : option IdInfo.IdInfo -> Var.Id -> Var.Id :=
+  fun arg_0__ arg_1__ =>
+    match arg_0__, arg_1__ with
+    | Some new_info, id => lazySetIdInfo id new_info
+    | None, id => id
+    end.
+
+Definition zapInfo
+   : (IdInfo.IdInfo -> option IdInfo.IdInfo) -> Var.Id -> Var.Id :=
+  fun zapper id => maybeModifyIdInfo (zapper ((@Var.idInfo tt id))) id.
+
+Definition zapIdTailCallInfo : Var.Id -> Var.Id :=
+  zapInfo IdInfo.zapTailCallInfo.
+
+Definition zapJoinId : Var.Id -> Var.Id :=
+  fun jid =>
+    if isJoinId jid : bool
+    then zapIdTailCallInfo (Var.setIdDetails jid IdInfo.VanillaId) else
+    jid.
+
+Definition asJoinId_maybe : Var.Id -> option BasicTypes.JoinArity -> Var.Id :=
+  fun arg_0__ arg_1__ =>
+    match arg_0__, arg_1__ with
+    | id, Some arity => asJoinId id arity
+    | id, None => zapJoinId id
+    end.
+
+Definition zapIdUsageInfo : Var.Id -> Var.Id :=
+  zapInfo IdInfo.zapUsageInfo.
+
+Definition zapIdUsedOnceInfo : Var.Id -> Var.Id :=
+  zapInfo IdInfo.zapUsedOnceInfo.
+
+Definition zapLamIdInfo : Var.Id -> Var.Id :=
+  zapInfo IdInfo.zapLamInfo.
+
+Definition setIdInfo : Var.Id -> IdInfo.IdInfo -> Var.Id :=
+  fun id info => lazySetIdInfo id info.
+
+Definition modifyIdInfo
+   : (IdInfo.IdInfo -> IdInfo.IdInfo) -> Var.Id -> Var.Id :=
+  fun fn id => setIdInfo id (fn ((@Var.idInfo tt id))).
+
+Definition modifyInlinePragma
+   : Var.Id -> (BasicTypes.InlinePragma -> BasicTypes.InlinePragma) -> Var.Id :=
+  fun id fn =>
+    modifyIdInfo (fun info =>
+                    IdInfo.setInlinePragInfo info (fn (IdInfo.inlinePragInfo info))) id.
+
+Definition setInlineActivation : Var.Id -> BasicTypes.Activation -> Var.Id :=
+  fun id act =>
+    modifyInlinePragma id (fun prag =>
+                             BasicTypes.setInlinePragmaActivation prag act).
+
+Definition setIdArity : Var.Id -> BasicTypes.Arity -> Var.Id :=
+  fun id arity =>
+    modifyIdInfo (fun arg_0__ => IdInfo.setArityInfo arg_0__ arity) id.
+
+Definition setIdCafInfo : Var.Id -> IdInfo.CafInfo -> Var.Id :=
+  fun id caf_info =>
+    modifyIdInfo (fun arg_0__ => IdInfo.setCafInfo arg_0__ caf_info) id.
+
+Definition setIdCallArity : Var.Id -> BasicTypes.Arity -> Var.Id :=
+  fun id arity =>
+    modifyIdInfo (fun arg_0__ => IdInfo.setCallArityInfo arg_0__ arity) id.
+
+Definition setIdDemandInfo : Var.Id -> Demand.Demand -> Var.Id :=
+  fun id dmd => modifyIdInfo (fun arg_0__ => arg_0__) id.
+
+Definition setIdOccInfo : Var.Id -> BasicTypes.OccInfo -> Var.Id :=
+  fun id occ_info =>
+    modifyIdInfo (fun arg_0__ => IdInfo.setOccInfo arg_0__ occ_info) id.
+
+Definition zapIdOccInfo : Var.Id -> Var.Id :=
+  fun b => setIdOccInfo b BasicTypes.noOccInfo.
+
+Definition setIdOneShotInfo : Var.Id -> BasicTypes.OneShotInfo -> Var.Id :=
+  fun id one_shot =>
+    modifyIdInfo (fun arg_0__ => IdInfo.setOneShotInfo arg_0__ one_shot) id.
+
+Definition updOneShotInfo : Var.Id -> BasicTypes.OneShotInfo -> Var.Id :=
+  fun id one_shot =>
+    let do_upd :=
+      match pair (idOneShotInfo id) one_shot with
+      | pair BasicTypes.NoOneShotInfo _ => true
+      | pair BasicTypes.OneShotLam _ => false
+      end in
+    if do_upd : bool then setIdOneShotInfo id one_shot else
+    id.
+
+Definition setIdSpecialisation : Var.Id -> IdInfo.RuleInfo -> Var.Id :=
+  fun id spec_info =>
+    modifyIdInfo (fun arg_0__ => IdInfo.setRuleInfo arg_0__ spec_info) id.
+
+Definition setIdStrictness : Var.Id -> Demand.StrictSig -> Var.Id :=
+  fun id sig => modifyIdInfo (fun arg_0__ => arg_0__) id.
+
+Definition setInlinePragma : Var.Id -> BasicTypes.InlinePragma -> Var.Id :=
+  fun id prag =>
+    modifyIdInfo (fun arg_0__ => IdInfo.setInlinePragInfo arg_0__ prag) id.
+
+Definition setOneShotLambda : Var.Id -> Var.Id :=
+  fun id =>
+    modifyIdInfo (fun arg_0__ =>
+                    IdInfo.setOneShotInfo arg_0__ BasicTypes.OneShotLam) id.
+
+Definition transferPolyIdInfo : Var.Id -> list Var.Var -> Var.Id -> Var.Id :=
+  fun old_id abstract_wrt new_id =>
+    let old_info := (@Var.idInfo tt old_id) in
+    let old_arity := IdInfo.arityInfo old_info in
+    let old_inline_prag := IdInfo.inlinePragInfo old_info in
+    let old_occ_info := IdInfo.occInfo old_info in
+    let new_occ_info := BasicTypes.zapOccTailCallInfo old_occ_info in
+    let old_strictness := IdInfo.strictnessInfo old_info in
+    let arity_increase := Util.count Var.isId abstract_wrt in
+    let new_arity := old_arity GHC.Num.+ arity_increase in
+    let new_strictness := tt in
+    let transfer :=
+      fun new_info =>
+        IdInfo.setOccInfo (IdInfo.setInlinePragInfo (IdInfo.setArityInfo new_info
+                                                                         new_arity) old_inline_prag) new_occ_info in
+    modifyIdInfo transfer new_id.
+
+Definition zapIdStrictness : Var.Id -> Var.Id :=
+  fun id => modifyIdInfo (fun arg_0__ => arg_0__) id.
+
+Definition clearOneShotLambda : Var.Id -> Var.Id :=
+  fun id =>
+    modifyIdInfo (fun arg_0__ =>
+                    IdInfo.setOneShotInfo arg_0__ BasicTypes.NoOneShotInfo) id.
+
+Definition mkExportedLocalId
+   : IdInfo.IdDetails -> Name.Name -> unit -> Var.Id :=
+  fun details name ty =>
+    Var.mkExportedLocalVar details name ty IdInfo.vanillaIdInfo.
+
+Definition mkExportedVanillaId : Name.Name -> unit -> Var.Id :=
+  fun name ty =>
+    Var.mkExportedLocalVar IdInfo.VanillaId name ty IdInfo.vanillaIdInfo.
+
+Definition mkGlobalId
+   : IdInfo.IdDetails -> Name.Name -> unit -> IdInfo.IdInfo -> Var.Id :=
+  Var.mkGlobalVar.
+
+Definition mkVanillaGlobalWithInfo
+   : Name.Name -> unit -> IdInfo.IdInfo -> Var.Id :=
+  mkGlobalId IdInfo.VanillaId.
+
+Definition mkVanillaGlobal : Name.Name -> unit -> Var.Id :=
+  fun name ty => mkVanillaGlobalWithInfo name ty IdInfo.vanillaIdInfo.
+
+Definition mkLocalIdOrCoVarWithInfo
+   : Name.Name -> unit -> IdInfo.IdInfo -> Var.Id :=
+  fun name ty info =>
+    let details := IdInfo.VanillaId in Var.mkLocalVar details name ty info.
+
+Definition mkLocalIdWithInfo : Name.Name -> unit -> IdInfo.IdInfo -> Var.Id :=
+  fun name ty info => Var.mkLocalVar IdInfo.VanillaId name ty info.
+
+Definition mkLocalId : Name.Name -> unit -> Var.Id :=
+  fun name ty => mkLocalIdWithInfo name ty IdInfo.vanillaIdInfo.
+
+Definition mkLocalIdOrCoVar : Name.Name -> unit -> Var.Id :=
+  fun name ty => mkLocalId name ty.
+
+Definition mkSysLocalOrCoVar
+   : FastString.FastString -> Unique.Unique -> unit -> Var.Id :=
+  fun fs uniq ty => mkLocalIdOrCoVar (Name.mkSystemVarName uniq fs) ty.
+
+Definition mkSysLocalOrCoVarM {m} `{UniqSupply.MonadUnique m}
+   : FastString.FastString -> unit -> m Var.Id :=
+  fun fs ty =>
+    UniqSupply.getUniqueM GHC.Base.>>=
+    (fun uniq => GHC.Base.return_ (mkSysLocalOrCoVar fs uniq ty)).
+
+Definition mkTemplateLocal : GHC.Num.Int -> unit -> Var.Id :=
+  fun i ty =>
+    mkSysLocalOrCoVar (FastString.fsLit (GHC.Base.hs_string__ "v"))
+    (Unique.mkBuiltinUnique i) ty.
+
+Definition mkTemplateLocalsNum : GHC.Num.Int -> list unit -> list Var.Id :=
+  fun n tys =>
+    GHC.List.zipWith mkTemplateLocal (GHC.Enum.enumFromTo n (GHC.List.length tys))
+    tys.
+
+Definition mkTemplateLocals : list unit -> list Var.Id :=
+  mkTemplateLocalsNum #1.
+
+Definition mkUserLocalOrCoVar
+   : OccName.OccName -> Unique.Unique -> unit -> SrcLoc.SrcSpan -> Var.Id :=
+  fun occ uniq ty loc => mkLocalIdOrCoVar (Name.mkInternalName uniq occ loc) ty.
+
+Definition mkWorkerId : Unique.Unique -> Var.Id -> unit -> Var.Id :=
+  fun uniq unwrkr ty =>
+    mkLocalIdOrCoVar (Name.mkDerivedInternalName OccName.mkWorkerOcc uniq
+                      (Name.getName unwrkr)) ty.
+
+Definition mkSysLocal
+   : FastString.FastString -> Unique.Unique -> unit -> Var.Id :=
+  fun fs uniq ty =>
+    if false : bool
+    then (Panic.assertPanic (GHC.Base.hs_string__ "ghc/compiler/basicTypes/Id.hs")
+          #313)
+    else mkLocalId (Name.mkSystemVarName uniq fs) ty.
+
+Definition mkSysLocalM {m} `{UniqSupply.MonadUnique m}
+   : FastString.FastString -> unit -> m Var.Id :=
+  fun fs ty =>
+    UniqSupply.getUniqueM GHC.Base.>>=
+    (fun uniq => GHC.Base.return_ (mkSysLocal fs uniq ty)).
+
+Definition mkUserLocal
+   : OccName.OccName -> Unique.Unique -> unit -> SrcLoc.SrcSpan -> Var.Id :=
+  fun occ uniq ty loc =>
+    if false : bool
+    then (Panic.assertPanic (GHC.Base.hs_string__ "ghc/compiler/basicTypes/Id.hs")
+          #330)
+    else mkLocalId (Name.mkInternalName uniq occ loc) ty.
+
+Definition recordSelectorTyCon : Var.Id -> IdInfo.RecSelParent :=
+  fun id =>
+    match Var.idDetails id with
+    | IdInfo.RecSelId parent _ => parent
+    | _ => Panic.panic (GHC.Base.hs_string__ "recordSelectorTyCon")
+    end.
+
+Definition setCaseBndrEvald : DataCon.StrictnessMark -> Var.Id -> Var.Id :=
+  fun str id => if DataCon.isMarkedStrict str : bool then id else id.
+
+Definition setIdExported : Var.Id -> Var.Id :=
+  Var.setIdExported.
+
+Definition setIdName : Var.Id -> Name.Name -> Var.Id :=
+  Var.setVarName.
+
+Definition setIdNotExported : Var.Id -> Var.Id :=
+  Var.setIdNotExported.
+
+Definition setIdType : Var.Id -> unit -> Var.Id :=
+  fun id ty => Var.setVarType id ty.
+
+Definition setIdUnique : Var.Id -> Unique.Unique -> Var.Id :=
+  Var.setVarUnique.
+
+Definition stateHackOneShot : BasicTypes.OneShotInfo :=
+  BasicTypes.OneShotLam.
 
 (* External variables:
-     bool list option unit BasicTypes.Activation BasicTypes.Arity
-     BasicTypes.InlinePragma BasicTypes.JoinArity BasicTypes.OccInfo
-     BasicTypes.OneShotInfo BasicTypes.RepArity CoreSyn.Unfolding
-     DataCon.StrictnessMark Demand.Demand Demand.StrictSig FastString.FastString
-     GHC.Num.Int IdInfo.CafInfo IdInfo.IdDetails IdInfo.IdInfo IdInfo.RecSelParent
-     IdInfo.RuleInfo Module.Module Name.Name OccName.OccName SrcLoc.SrcSpan
-     UniqSupply.MonadUnique Unique.Unique Var.Id Var.JoinId Var.Var
+     None Some andb bool false list lookupClass lookupDataCon negb option orb pair
+     true tt unit BasicTypes.Activation BasicTypes.Arity BasicTypes.InlinePragma
+     BasicTypes.JoinArity BasicTypes.NoOneShotInfo BasicTypes.OccInfo
+     BasicTypes.OneShotInfo BasicTypes.OneShotLam BasicTypes.RuleMatchInfo
+     BasicTypes.inlinePragmaActivation BasicTypes.inlinePragmaRuleMatchInfo
+     BasicTypes.isConLike BasicTypes.isDeadOcc BasicTypes.isOneOcc
+     BasicTypes.noOccInfo BasicTypes.occ_in_lam BasicTypes.setInlinePragmaActivation
+     BasicTypes.zapOccTailCallInfo Class.Class DataCon.DataCon DataCon.StrictnessMark
+     DataCon.isMarkedStrict DataCon.isUnboxedSumCon DataCon.isUnboxedTupleCon
+     Datatypes.id Demand.Demand Demand.StrictSig FastString.FastString
+     FastString.fsLit GHC.Base.mappend GHC.Base.op_zgzgze__ GHC.Base.return_
+     GHC.Enum.enumFromTo GHC.List.length GHC.List.zipWith GHC.Num.Int
+     GHC.Num.fromInteger GHC.Num.op_zp__ IdInfo.CafInfo IdInfo.ClassOpId
+     IdInfo.DFunId IdInfo.DataConWorkId IdInfo.DataConWrapId IdInfo.FCallId
+     IdInfo.IdDetails IdInfo.IdInfo IdInfo.JoinId IdInfo.PrimOpId IdInfo.RecSelData
+     IdInfo.RecSelId IdInfo.RecSelParent IdInfo.RecSelPatSyn IdInfo.RuleInfo
+     IdInfo.VanillaId IdInfo.arityInfo IdInfo.cafInfo IdInfo.callArityInfo
+     IdInfo.inlinePragInfo IdInfo.isEmptyRuleInfo IdInfo.occInfo IdInfo.oneShotInfo
+     IdInfo.ruleInfo IdInfo.setArityInfo IdInfo.setCafInfo IdInfo.setCallArityInfo
+     IdInfo.setInlinePragInfo IdInfo.setOccInfo IdInfo.setOneShotInfo
+     IdInfo.setRuleInfo IdInfo.strictnessInfo IdInfo.vanillaIdInfo IdInfo.zapLamInfo
+     IdInfo.zapTailCallInfo IdInfo.zapUsageInfo IdInfo.zapUsedOnceInfo Maybes.orElse
+     Module.Module Name.Name Name.getName Name.isInternalName Name.localiseName
+     Name.mkDerivedInternalName Name.mkInternalName Name.mkSystemVarName
+     Name.nameIsLocalOrFrom OccName.OccName OccName.mkWorkerOcc Panic.assertPanic
+     Panic.noString Panic.panic Panic.panicStr Panic.someSDoc Panic.warnPprTrace
+     SrcLoc.SrcSpan UniqSupply.MonadUnique UniqSupply.getUniqueM Unique.Unique
+     Unique.mkBuiltinUnique Util.count Var.Id Var.JoinId Var.Var Var.idDetails
+     Var.idInfo Var.isId Var.isLocalId Var.lazySetIdInfo Var.mkExportedLocalVar
+     Var.mkGlobalVar Var.mkLocalVar Var.setIdDetails Var.setIdExported
+     Var.setIdNotExported Var.setVarName Var.setVarType Var.setVarUnique Var.varName
+     Var.varType Var.varUnique
 *)
