examples/ghc/deps/Id.mk
@@ -1,1 +1,1 @@
-lib/Id.v: 
+lib/Id.v: lib/BasicTypes.h2ci lib/IdInfo.h2ci
